start otd proof

src/datalog/OperationalToDistributed.v
@@ -3,33 +3,33 @@ From Datalog Require Import Datalog Node Operational Smallstep Graph List Distri
 From coqutil Require Import Map.Interface Eqb Tactics.fwd Tactics.
 From coqutil Require Import Semantics.OmniSmallstepCombinators.
 Import ListNotations.
+Import node.
 
 Open Scope bool_scope.
 
-#[local] Instance mf_label : mf_labelT := source.
+#[local] Instance sender_label : sender_labelT := source.
 Section __.
-  Context {rel : relT} {exprvar : exprvarT} {fn : fnT} {aggregator : aggregatorT} {T : valueT}.
+  Context `{params : datalog_params}.
   Context {rel_eqb : Eqb rel} {rel_eqb_ok : Eqb_ok rel_eqb}.
   Context {rule_eqb : Eqb rule} {rule_eqb_ok : Eqb_ok rule_eqb}.
-  Context {sig : signature fn aggregator T}.
-  Context {context : map.map exprvar T} {context_ok : map.ok context}.
   Context (is_input : rel -> bool).
-  Context (p : list rule).
-  Context (Hmeta_rules : meta_rules_valid p).
-  Context (Hp_rule_inputs : Forall (good_rule_inputs is_input) p).
+  Context (p : program).
+  Context (Hmeta_rules : program.meta_rules_valid p).
 
-  Context {gns_map : map.map node_id (graph_node_state dfact dfact_mod_count Node.node_state)}.
+  (* Context (Hp_rule_inputs : program.good_input_set p). *)
+
+  Context {gns_map : map.map node_id (graph_node_state node.message node.action_label node.state)}.
   Context {gns_map_ok : map.ok gns_map}.
 
   Context (rel_forward : source -> destn -> rel -> bool).
-  Context {prog_map : map.map node_id (list rule)} {prog_map_ok : map.ok prog_map}.
-  Context {sent_map : map.map rule (list (dfact (mf_label := op_source)))}.
+  Context {prog_map : map.map node_id program} {prog_map_ok : map.ok prog_map}.
+  Context {sent_map : map.map rule (list (message (sender_label := op_source)))}.
   Context (graph_prog : prog_map).
 
-  Local Notation R_senders := (Operational.R_senders is_input p).
-  Local Notation ok_to_deduce_fact := (Node.ok_to_deduce_fact R_senders).
-  Local Notation new_facts := (Node.new_facts R_senders).
-  Local Notation fire_at_rule := (Operational.fire_at_rule is_input p).
+  Local Abbreviation R_senders := (Operational.R_senders is_input p).
+  (* Local Notation ok_to_deduce_fact := (Node.ok_to_deduce_fact R_senders). *)
+  (* Local Notation new_facts := (Node.new_facts R_senders). *)
+  (* Local Notation fire_at_rule := (Operational.fire_at_rule is_input p). *)
 
   Context (graph_senders : rel -> list source).
 
@@ -38,25 +38,26 @@ Section __.
   Local Notation comp_step := (Operational.comp_step is_input p).
   Local Notation has_derived_datalog_fact := (Operational.has_derived_datalog_fact is_input p).
 
-  Definition graph_prog_distributes_normal_rules (rules : list rule) :=
-    forall r,
-      is_normal r = true ->
-      In r rules <-> In r (concat (values graph_prog)).
+  Definition normal_rules_of :=
+    concat (map program.rules (values graph_prog)).
 
-  Definition graph_prog_distributes_meta_rules (rules : list rule) :=
-    forall concls hyps,
-      In (meta_rule concls hyps) rules ->
-      Forall_map (fun _ rules =>
+  Definition enough_meta_rules (p : program) :=
+    forall mr,
+      In mr p.(program.meta_rules) ->
+      Forall_map (fun _ np =>
                     forall R,
-                      In R (map meta_clause.rel concls) ->
-                      In R (flat_map concl_rels (filter is_normal rules)) ->
-                      In (meta_rule concls hyps) rules)
+                      In R (map clause_pattern.rel mr.(meta_rule.concls)) ->
+                      In R (flat_map rule.concl_rels p.(program.rules)) ->
+                      In mr np.(program.meta_rules))
         graph_prog.
+
+  Definition meta_rules_of :=
+    concat (map program.meta_rules (values graph_prog)).
 
   Definition node_senders_ok :=
     forall R n np,
       map.get graph_prog n = Some np ->
-      In R (flat_map concl_rels np) ->
+      In R (program.concl_rels np) ->
       In (node_source n) (graph_senders R).
 
   Definition input_senders_ok :=
@@ -64,23 +65,32 @@ Section __.
       is_input R = true ->
       In input_source (graph_senders R).
 
-  Context (Hlayout_normal : graph_prog_distributes_normal_rules p).
-  Context (Hlayout_meta : graph_prog_distributes_meta_rules p).
+  Context (Hlayout_normal : same_set p.(program.rules) normal_rules_of).
+  Context (Hlayout_meta : same_set p.(program.meta_rules) meta_rules_of).
   Context (Hsenders_node : node_senders_ok).
   Context (Hsenders_input : input_senders_ok).
 
-  Definition distribute_R (os : state) (gs : graph_state dfact dfact_mod_count node_state) :=
+  Definition distribute_R (os : Operational.state) (gs : graph_state message action_label state) :=
     Forall2_map (fun n np ns =>
-                   Permutation (flat_map normal_facts_of (flat_map (get_or_default os.(sents)) (dedup np)))
-                     (flat_map normal_facts_of ns.(gns_node_state).(Node.sent_facts)) /\
-                     (forall R args num,
-                         In (meta_dfact R args (node_source n) num) ns.(gns_node_state).(Node.sent_facts) <->
+                   Permutation
+                     (flat_map message.normal_facts (flat_map (get_or_default os.(sents)) (dedup np.(program.rules))))
+                     (flat_map message.normal_facts ns.(gns_node_state).(state.sent)) /\
+                     (forall pat num,
+                         In (message.done_with pat (node_source n) num) ns.(gns_node_state).(state.sent) <->
                            (exists nums,
-                               Forall2 (fun nr num0 => In (meta_dfact R args (from_rule nr) num0) (get_or_default os.(sents) nr))
-                                 (dedup (filter is_normal np)) nums /\
+                               Forall2 (fun nr num0 => In (message.done_with pat (from_rule nr) num0) (get_or_default os.(sents) nr))
+                                 (dedup np.(program.rules)) nums /\
                                  num = list_sum nums)) /\
                      ns.(gns_queue) = [])
       graph_prog gs.(graph_nodes).
+
+  Lemma can_deduce_iff os gs n ns np f r :
+    distribute_R os gs ->
+    map.get gs.(graph_nodes) n = Some ns ->
+    map.get graph_prog n = Some np ->
+    can_deduce graph_senders np (node_source n) ns.(gns_node_state) (message.normal f) <->
+      fire_at_rule is_input p r os.(known_facts) (get_or_default os.(sents) r) (message.normal f).
+  Proof. Admitted.
 
   Lemma sim1 os gs os' :
     distribute_R os gs ->
@@ -90,23 +100,27 @@ Section __.
         distribute_R os' gs'.
   Proof.
     intros H. invert 1. rename H1 into Hp, H2 into Hr.
-    cbv [fire_at_rule] in Hr. fwd.
-    cbv [can_fire_rule_at] in Hrp0. destruct Hrp0 as [Hrp0|Hrp0].
-    - subst. cbv [non_meta_rules] in Hp. apply filter_In in Hp. fwd.
-      clear Hrp2. cbv [can_deduce_fact] in Hrp1. Tactics.destruct_one_match_hyp.
-      2: { fwd. simpl in *. discriminate. }
-      fwd.
-      cbv [graph_prog_distributes_normal_rules] in Hlayout_normal.
-      apply Hlayout_normal in Hpp0; auto. apply in_concat in Hpp0. fwd.
-      apply In_values in Hpp0p0. fwd.
-      cbv [distribute_R] in H.
+    cbv [fire_at_rule] in Hr. cbv [can_deduce] in Hr.
+    destruct new_fact as [nf|pat src num]; fwd; simpl in *.
+    - destruct Hrp0p0; contradiction || subst.
+      apply Hlayout_normal in Hp. cbv [normal_rules_of] in Hp.
+      apply in_concat in Hp. fwd. apply in_map_iff in Hpp0. fwd.
+      apply In_values in Hpp0p1. fwd.
       epose proof Forall2_map_get_l as Hk. especialize Hk; try eassumption. fwd.
-      do 2 eexists. split.
+      cbv [distribute_R] in H. do 2 eexists. split.
       + eapply star_step.
         -- apply star_one. apply gstep_run.
            ++ eassumption.
            ++ cbv [prog_at]. erewrite get_or_default_Some by eassumption.
-              apply node_deduce_step.
+              eapply node.deduce_step with (output := message.normal _).
+              simpl. split.
+              --- apply Exists_exists. eexists. split; [eassumption|].
+                  Print can_deduce.
+                  move Hrp0p1 at bottom. cbv [can_deduce_normal_fact] in Hrp0p1.
+                  fwd. cbv [can_deduce_normal_fact]. eexists. split; [eassumption|].
+                  About R_senders.
+                  Print can_deduce_normal_fact.
+                  Search @graph_senders.
               cbv [Node.new_facts]. Print can_deduce_fact.
               Print node_step.
         destruct r; simpl in *; try discriminate; fwd. 2: { simpl in *.
